Makefile
@@ -1,0 +1,9 @@
+.PHONY: rocq clean
+
+ROCQC=rocq compile
+
+rocq:
+	$(ROCQC) LZ.v
+
+clean:
+	rm -f *.vo* *.glob *.aux .*.aux .*.cache
