README.md
@@ -1,0 +1,2 @@
+# Formal Verification of the LZ77 Compression Algorithm
+
